Added most of the proof end-to-mid :) Hacked a free variable into the existing code (for the previous value of x10)

examples/riscv/incr/incr_propScript.sml
@@ -27,7 +27,13 @@ open symb_prop_transferTheory;
 
 open jgmt_rel_bir_contTheory;
 
+open bir_symbTheory;
 open birs_stepLib;
+open bir_symb_sound_coreTheory;
+open symb_recordTheory;
+open symb_interpretTheory;
+
+open pred_setTheory;
 
 open incrTheory;
 
@@ -46,11 +52,19 @@ Definition riscv_incr_post_def:
 End
 
 Definition bir_incr_pre_def:
-  bir_incr_pre : bir_exp_t = bir_exp_true (* FIXME *)
+  bir_incr_pre x : bir_exp_t =
+  BExp_BinPred
+    BIExp_Equal
+    (BExp_Den (BVar "x10" (BType_Imm Bit64)))
+    (BExp_Const (Imm64 x))
 End
 
 Definition bir_incr_post_def:
- bir_incr_post : bir_exp_t = bir_exp_true (* FIXME *)
+ bir_incr_post x : bir_exp_t =
+  BExp_BinPred
+    BIExp_Equal
+    (BExp_Den (BVar "x10" (BType_Imm Bit64)))
+    (BExp_Const (Imm64 (x + 1w)))
 End
 
 (* ------ *)
@@ -62,28 +76,28 @@ Definition incr_analysis_L_def:
 End
 
 val birs_state_init_lbl = ``<|bpc_label := BL_Address (Imm64 0w); bpc_index := 0|>``;
-val birs_state_end_lbl = (snd o dest_eq o concl o EVAL) ``bir_block_pc (BL_Address (Imm64 8w))``;
+val birs_state_end_lbl = (snd o dest_eq o concl o EVAL) ``bir_block_pc (BL_Address (Imm64 4w))``;
 
 Definition bprecond_def:
-  bprecond = bir_exp_true
+  bprecond = bir_incr_pre
 End
 
 val bprecond = (fst o dest_eq o concl) bprecond_def;
 
 Definition bsysprecond_def:
-  bsysprecond = FST (THE (birs_eval_exp ^bprecond (bir_senv_GEN_list birenvtyl_riscv)))
+  bsysprecond x = FST (THE (birs_eval_exp (^bprecond x) (bir_senv_GEN_list birenvtyl_riscv)))
 End
 
 Theorem bprecond_birs_eval_exp_thm = (computeLib.RESTR_EVAL_CONV [``birs_eval_exp``] THENC
    birs_stepLib.birs_eval_exp_CONV)
-     ``birs_eval_exp bprecond (bir_senv_GEN_list birenvtyl_riscv)``
+     ``birs_eval_exp (bprecond x) (bir_senv_GEN_list birenvtyl_riscv)``
 
 Theorem bsysprecond_thm =
- (REWRITE_CONV [bsysprecond_def, birs_eval_exp_ALT_thm, bprecond_birs_eval_exp_thm] THENC EVAL) ``bsysprecond``
+ (REWRITE_CONV [bsysprecond_def, birs_eval_exp_ALT_thm, bprecond_birs_eval_exp_thm] THENC EVAL) ``bsysprecond x``
 
-Theorem bprecond_birs_eval_exp_thm2 = REWRITE_CONV [bprecond_birs_eval_exp_thm, GSYM bsysprecond_thm] ``birs_eval_exp bprecond (bir_senv_GEN_list birenvtyl_riscv)``
+Theorem bprecond_birs_eval_exp_thm2 = REWRITE_CONV [bprecond_birs_eval_exp_thm, GSYM bsysprecond_thm] ``birs_eval_exp (bprecond x) (bir_senv_GEN_list birenvtyl_riscv)``
 
-val bsysprecond = (fst o dest_eq o concl) bsysprecond_def;
+val bsysprecond = (fst o dest_eq o concl o Q.SPEC `pre_x10`) bsysprecond_def;
 
 val birs_state_init_pre = ``<|
   bsst_pc       := ^birs_state_init_lbl;
@@ -122,28 +136,28 @@ val birs_prop_transfer_thm =
   (MATCH_MP symb_prop_transferTheory.symb_prop_transfer_thm birs_symb_symbols_f_sound_prog_thm);
 
 Definition bprog_P_def:
-  bprog_P ((SymbConcSt pc st status):(bir_programcounter_t, string, bir_val_t, bir_status_t) symb_concst_t) =
+  bprog_P x ((SymbConcSt pc st status):(bir_programcounter_t, string, bir_val_t, bir_status_t) symb_concst_t) =
       (status = BST_Running /\
        pc.bpc_index = 0 /\
        bir_envty_list birenvtyl_riscv st /\
-       bir_eval_exp ^bprecond (BEnv st) = SOME bir_val_true)
+       bir_eval_exp (^bprecond x) (BEnv st) = SOME bir_val_true)
 End
 
 (* translate the property to BIR state property *)
 Theorem bprog_P_thm:
-  !bs.
-  bprog_P (birs_symb_to_concst bs) =
+  !x bs.
+  bprog_P x (birs_symb_to_concst bs) =
       (bs.bst_status = BST_Running /\
        bs.bst_pc.bpc_index = 0 /\
        bir_envty_list_b birenvtyl_riscv bs.bst_environ /\
-       bir_eval_exp ^bprecond bs.bst_environ = SOME bir_val_true)
+       bir_eval_exp (^bprecond x) bs.bst_environ = SOME bir_val_true)
 Proof
  REPEAT STRIP_TAC >>
   FULL_SIMP_TAC (std_ss) [birs_symb_to_concst_def, bprog_P_def, bir_envty_list_b_thm, bir_BEnv_lookup_EQ_thm]
 QED
 
 Definition bprog_Q_def:
-  bprog_Q
+  bprog_Q x
      ((SymbConcSt pc1 st1 status1):(bir_programcounter_t, string, bir_val_t, bir_status_t) symb_concst_t)
      ((SymbConcSt pc2 st2 status2):(bir_programcounter_t, string, bir_val_t, bir_status_t) symb_concst_t)
     =
@@ -151,25 +165,295 @@ Definition bprog_Q_def:
        (pc2 = ^birs_state_end_lbl)
        /\
        (status2 = BST_Running)
+       /\
+       (st2 "x10" = SOME (BVal_Imm (Imm64 (x + 1w))))
      )
 End
 
 Theorem bprog_Q_thm:
-  !bs1 bs2.
-  bprog_Q (birs_symb_to_concst bs1) (birs_symb_to_concst bs2) =
+  !x bs1 bs2.
+  bprog_Q x (birs_symb_to_concst bs1) (birs_symb_to_concst bs2) =
     (
       (bs2.bst_pc = ^birs_state_end_lbl)
       /\
       (bs2.bst_status = BST_Running)
+      /\
+      (bir_env_lookup "x10" bs2.bst_environ = SOME (BVal_Imm (Imm64 (x + 1w))))
     )
 Proof
 FULL_SIMP_TAC (std_ss) [birs_symb_to_concst_def, bprog_Q_def]
 QED
+(* ........................... *)
+
+(* P is generic enough *)
+
+Theorem bprog_P_entails_thm:
+  P_entails_an_interpret (bir_symb_rec_sbir ^bprog_tm) (bprog_P pre_x10) (birs_symb_to_symbst ^birs_state_init_pre)
+Proof
+FULL_SIMP_TAC (std_ss++birs_state_ss) [P_entails_an_interpret_def] >>
+  REPEAT STRIP_TAC >>
+
+  ASSUME_TAC ((GSYM o Q.SPEC `s`) birs_symb_to_concst_EXISTS_thm) >>
+  FULL_SIMP_TAC (std_ss++birs_state_ss) [birs_symb_matchstate_EQ_thm] >>
+
+  FULL_SIMP_TAC (std_ss++birs_state_ss) [birs_symb_to_symbst_def, symb_symbst_pc_def] >>
+
+  Cases_on `s` >> Cases_on `st` >>
+  FULL_SIMP_TAC (std_ss++holBACore_ss++symb_typesLib.symb_TYPES_ss) [bprog_P_def, birs_symb_to_concst_def, symb_concst_pc_def] >>
+
+  Cases_on `b0` >>
+  FULL_SIMP_TAC (std_ss) [bir_envTheory.bir_env_lookup_def] >>
+  PAT_X_ASSUM ``A = (\B. C)`` (ASSUME_TAC o GSYM) >>
+  FULL_SIMP_TAC (std_ss) [boolTheory.ETA_THM] >>
+
+  `(ALL_DISTINCT (MAP FST birenvtyl_riscv))` by EVAL_TAC >>
+
+  METIS_TAC [bprog_P_entails_gen_thm, birenvtyl_EVAL_thm, bprecond_birs_eval_exp_thm2]
+QED
+
+(* ........................... *)
+
+
+Theorem bir_Pi_overapprox_Q_thm:
+  !p P sys Pi Q.
+  (Pi_overapprox_Q (bir_symb_rec_sbir p) P (birs_symb_to_symbst sys) (IMAGE birs_symb_to_symbst Pi) Q)
+  <=>
+  (!sys2 bs bs' H.
+     sys2 IN Pi ==>
+     birs_symb_matchstate sys H bs ==>
+     (\bs. P (birs_symb_to_concst bs)) bs ==>
+     (?H'. symb_interpr_ext H' H /\ birs_symb_matchstate sys2 H' bs') ==>
+     (\bs bs'. Q (birs_symb_to_concst bs) (birs_symb_to_concst bs')) bs bs')
+Proof
+FULL_SIMP_TAC (std_ss++birs_state_ss) [Pi_overapprox_Q_def] >>
+  REPEAT STRIP_TAC >>
+
+  FULL_SIMP_TAC (std_ss) [symb_matchstate_ext_def, birs_symb_matchstate_EQ_thm] >>
+
+  EQ_TAC >- (
+    REPEAT STRIP_TAC >>
+    PAT_X_ASSUM ``!x.A`` (ASSUME_TAC o Q.SPECL [`birs_symb_to_symbst sys2`, `birs_symb_to_concst bs`, `birs_symb_to_concst bs'`, `H`]) >>
+
+    REV_FULL_SIMP_TAC (std_ss) [IMAGE_IN, symb_matchstate_ext_def, birs_symb_matchstate_EQ_thm] >>
+    METIS_TAC []
+  ) >>
+
+  REPEAT STRIP_TAC >>
+
+  `?bsys. sys' = birs_symb_to_symbst bsys` by (
+    METIS_TAC [birs_symb_to_symbst_EXISTS_thm]
+  ) >>
+  `?bs.  s  = birs_symb_to_concst bs /\
+   ?bs'. s' = birs_symb_to_concst bs'` by (
+    METIS_TAC [birs_symb_to_concst_EXISTS_thm]
+  ) >>
+
+  PAT_X_ASSUM ``!x.A`` (ASSUME_TAC o Q.SPECL [`bsys`, `bs`, `bs'`, `H`]) >>
+
+  `bsys IN Pi` by (
+    FULL_SIMP_TAC std_ss [] >>
+
+    `birs_symb_from_symbst o birs_symb_to_symbst = I` by (
+      SIMP_TAC std_ss [combinTheory.o_DEF, bir_symbTheory.birs_symb_to_from_symbst_thm] >>
+      MATCH_MP_TAC boolTheory.EQ_EXT >>
+      SIMP_TAC std_ss [combinTheory.I_THM]
+    ) >>
+    METIS_TAC [IMAGE_IN, IMAGE_IMAGE, bir_symbTheory.birs_symb_to_from_symbst_thm, IMAGE_I]
+  ) >>
+
+  FULL_SIMP_TAC (std_ss) [symb_matchstate_ext_def, birs_symb_matchstate_EQ_thm] >>
+  REV_FULL_SIMP_TAC (std_ss) [symb_matchstate_ext_def, birs_symb_matchstate_EQ_thm] >>
+  METIS_TAC []
+QED
+
+
+(* Q is implied by sys and Pi *)
+Theorem bprog_Pi_overapprox_Q_thm:
+  Pi_overapprox_Q (bir_symb_rec_sbir ^bprog_tm) (bprog_P pre_x10) (birs_symb_to_symbst ^birs_state_init_pre) ^Pi_f(*(IMAGE birs_symb_to_symbst {a;b;c;d})*) (bprog_Q pre_x10)
+Proof
+REWRITE_TAC [bir_Pi_overapprox_Q_thm] >>
+  REPEAT GEN_TAC >>
+
+  REWRITE_TAC [pred_setTheory.IMAGE_INSERT, pred_setTheory.IMAGE_EMPTY, pred_setTheory.IN_INSERT, pred_setTheory.NOT_IN_EMPTY] >>
+  STRIP_TAC >> (
+    POP_ASSUM (fn thm => (ASSUME_TAC thm >> Q.ABBREV_TAC `sys3 = ^((snd o dest_eq o concl) thm)`)) >>
+    ASM_SIMP_TAC std_ss [] >>
+    rename1 `sys4 = sys3` >>
+    rename1 `sys4 = sys2` >>
+    PAT_X_ASSUM ``A = B`` (K ALL_TAC) >>
+
+    DISCH_TAC >>
+    POP_ASSUM (fn thm => (ASSUME_TAC thm >> Q.ABBREV_TAC `sys1 = ^((snd o dest_comb o fst o dest_comb o fst o dest_comb o concl) thm)`)) >>
+    POP_ASSUM (fn thm0 => POP_ASSUM (fn thm1 => (ASSUME_TAC thm0 >> ASSUME_TAC thm1))) >>
+    REPEAT STRIP_TAC >>
+
+    (* now the proof state is somewhat clean *)
+
+    FULL_SIMP_TAC (std_ss) [bprog_Q_thm] >>
+    (* pc *)
+    CONJ_TAC >- (
+      Q.UNABBREV_TAC `sys2` >>
+      FULL_SIMP_TAC (std_ss++birs_state_ss) [birs_symb_matchstate_def]
+    ) >>
+    (* status Running *)
+    CONJ_TAC >- (
+      Q.UNABBREV_TAC `sys2` >>
+      FULL_SIMP_TAC (std_ss++birs_state_ss) [birs_symb_matchstate_def]
+    ) >>
+
+    (* the property (here: pre_x10 + 1) *)
+    `BVar "sy_x10" (BType_Imm Bit64) IN symb_interpr_dom H` by (
+      `symb_interpr_for_symbs (birs_symb_symbols sys1) H` by (
+        FULL_SIMP_TAC (std_ss++birs_state_ss) [birs_symb_matchstate_def]
+      ) >>
+
+      Q.UNABBREV_TAC `sys1` >>
+      POP_ASSUM (ASSUME_TAC o CONV_RULE (
+          REWRITE_CONV [bsysprecond_thm, birenvtyl_EVAL_thm] THENC
+          computeLib.RESTR_EVAL_CONV [``birs_symb_symbols``] THENC
+          aux_setLib.birs_symb_symbols_MATCH_CONV)
+        ) >>
+
+      FULL_SIMP_TAC (std_ss) [symb_interpr_for_symbs_def, INSERT_SUBSET]
+    ) >>
+    `BVar "sy_x10" (BType_Imm Bit64) IN symb_interpr_dom H'` by (
+      `symb_interpr_for_symbs (birs_symb_symbols sys2) H'` by (
+        FULL_SIMP_TAC (std_ss++birs_state_ss) [birs_symb_matchstate_def]
+      ) >>
+
+      Q.UNABBREV_TAC `sys2` >>
+      POP_ASSUM (ASSUME_TAC o CONV_RULE (
+          REWRITE_CONV [bsysprecond_thm, birenvtyl_EVAL_thm] THENC
+          computeLib.RESTR_EVAL_CONV [``birs_symb_symbols``] THENC
+          aux_setLib.birs_symb_symbols_MATCH_CONV)
+        ) >>
+
+      FULL_SIMP_TAC (std_ss) [symb_interpr_for_symbs_def, INSERT_SUBSET]
+    ) >>
+
+    `symb_interpr_get H' (BVar "sy_x10" (BType_Imm Bit64)) = symb_interpr_get H (BVar "sy_x10" (BType_Imm Bit64))` by (
+      FULL_SIMP_TAC std_ss [symb_interpr_ext_def, symb_interprs_eq_for_def]
+    ) >>
+
+    `bir_eval_exp (bprecond pre_x10) bs.bst_environ = SOME bir_val_true` by (
+      Q.UNABBREV_TAC `sys1` >>
+      FULL_SIMP_TAC (std_ss) [bprog_P_thm]
+    ) >>
+
+    (* use bprog_P *)
+    `symb_interpr_get H (BVar "sy_x10" (BType_Imm Bit64)) = SOME (BVal_Imm (Imm64 pre_x10))` by (
+      FULL_SIMP_TAC (std_ss) [bprog_P_thm] >>
+      `bir_env_lookup "x10" bs.bst_environ = SOME (BVal_Imm (Imm64 pre_x10))` by (
+        cheat
+      ) >>
+
+      cheat
+(*
+      Q.UNABBREV_TAC `sys1` >>
+      Q.UNABBREV_TAC `sys2` >>
+
+      FULL_SIMP_TAC (std_ss++birs_state_ss) [birs_symb_matchstate_def] >>
+
+      FULL_SIMP_TAC (std_ss++birs_state_ss) [birs_matchenv_def] >>
+      REPEAT (PAT_X_ASSUM ``!A.B`` (ASSUME_TAC o EVAL_RULE o Q.SPEC `"x10"`)) >>
+      FULL_SIMP_TAC (std_ss) [] >>
+
+      FULL_SIMP_TAC (std_ss++birs_state_ss) [birs_interpr_welltyped_def] >>
+      REPEAT (PAT_X_ASSUM ``!A.B`` (ASSUME_TAC o EVAL_RULE o Q.SPEC `BVar "sy_x10" (BType_Imm Bit64)`)) >>
+      FULL_SIMP_TAC (std_ss++holBACore_ss) [] >>
+      REV_FULL_SIMP_TAC (std_ss++holBACore_ss) [] >>
+
+      Cases_on `symb_interpr_get H (BVar "sy_x10" (BType_Imm Bit64))` >- (
+        METIS_TAC [symb_interpr_dom_IMP_get_CASES_thm, optionTheory.option_CLAUSES]
+      ) >>
+      FULL_SIMP_TAC (std_ss++holBACore_ss) [optionTheory.option_CLAUSES] >>
+
+      `bir_val_is_Imm_s Bit64 x` by (
+        METIS_TAC [bir_valuesTheory.bir_val_checker_TO_type_of]
+      ) >>
+      FULL_SIMP_TAC std_ss [bir_valuesTheory.bir_val_is_Imm_s_def, bir_immTheory.n2bs_def] >>
+
+      FULL_SIMP_TAC (std_ss++holBACore_ss) []
+*)
+    ) >>
+
+    (* *)
+    cheat
+(*
+    `(?v.
+       bir_env_lookup "countw" bs.bst_environ = SOME v /\
+       birs_interpret_fun H (THE (sys1.bsst_environ "countw")) = SOME v) /\
+     (?v'.
+       bir_env_lookup "countw" bs'.bst_environ = SOME v' /\
+       birs_interpret_fun H' (THE (sys2.bsst_environ "countw")) = SOME v')` by (
+      Q.UNABBREV_TAC `sys1` >>
+      Q.UNABBREV_TAC `sys2` >>
+
+      FULL_SIMP_TAC (std_ss++birs_state_ss) [birs_symb_matchstate_def] >>
+
+      FULL_SIMP_TAC (std_ss++birs_state_ss) [birs_matchenv_def] >>
+      REPEAT (PAT_X_ASSUM ``!A.B`` (ASSUME_TAC o EVAL_RULE o Q.SPEC `"countw"`)) >>
+      FULL_SIMP_TAC (std_ss) [] >>
+
+      FULL_SIMP_TAC (std_ss++birs_state_ss) [birs_interpr_welltyped_def] >>
+      REPEAT (PAT_X_ASSUM ``!A.B`` (ASSUME_TAC o EVAL_RULE o Q.SPEC `BVar "sy_countw" (BType_Imm Bit64)`)) >>
+      FULL_SIMP_TAC (std_ss++holBACore_ss) [] >>
+      REV_FULL_SIMP_TAC (std_ss++holBACore_ss) [] >>
+
+      Cases_on `symb_interpr_get H (BVar "sy_countw" (BType_Imm Bit64))` >- (
+        METIS_TAC [symb_interpr_dom_IMP_get_CASES_thm, optionTheory.option_CLAUSES]
+      ) >>
+      FULL_SIMP_TAC (std_ss++holBACore_ss) [optionTheory.option_CLAUSES] >>
+
+      FULL_SIMP_TAC (std_ss++holBACore_ss) [birs_auxTheory.birs_gen_env_GET_thm, birs_auxTheory.birs_gen_env_GET_NULL_thm] >>
+      ASM_REWRITE_TAC [birs_interpret_fun_def, birs_interpret_subst_def, birs_interpret_subst_fmap_def, bir_typing_expTheory.bir_vars_of_exp_def, bir_envTheory.bir_env_empty_def, bir_envTheory.bir_env_map_empty_def] >>
+
+      computeLib.RESTR_EVAL_TAC [``bir_exp_subst``] >>
+      ASM_REWRITE_TAC []
+    ) >>
+
+    REPEAT (PAT_X_ASSUM ``birs_symb_matchstate A B C`` (K ALL_TAC)) >>
+    Q.UNABBREV_TAC `sys1` >>
+    Q.UNABBREV_TAC `sys2` >>
+    FULL_SIMP_TAC (std_ss++birs_state_ss) [] >>
+    FULL_SIMP_TAC (std_ss++holBACore_ss) [birs_auxTheory.birs_gen_env_GET_thm, birs_auxTheory.birs_gen_env_GET_NULL_thm] >>
+    (* now the proof state is pretty much cleaned up *)
+
+    FULL_SIMP_TAC std_ss [birs_interpret_fun_thm] >>
+    REPEAT (PAT_X_ASSUM ``birs_interpret_fun_ALT A B = SOME C`` (ASSUME_TAC o computeLib.RESTR_EVAL_RULE [])) >>
+    FULL_SIMP_TAC std_ss [] >>
+    REV_FULL_SIMP_TAC std_ss [] >>
+    FULL_SIMP_TAC (std_ss++holBACore_ss) [] >>
+
+    PAT_X_ASSUM ``BVal_Imm (Imm64 A) = B`` (ASSUME_TAC o GSYM) >>
+    FULL_SIMP_TAC (std_ss++holBACore_ss) [] >>
+
+    (* still have to unpack the precondition for the space fact about countw *)
+    FULL_SIMP_TAC (std_ss++holBACore_ss) [bprecond_def] >>
+    REPEAT (PAT_X_ASSUM ``bir_eval_bin_exp BIExp_And A B = SOME bir_val_true`` (ASSUME_TAC o MATCH_MP birs_rulesTheory.bir_conj_true) >> FULL_SIMP_TAC std_ss []) >>
+    IMP_RES_TAC bir_env_read_countw_lookup_thm >>
+    FULL_SIMP_TAC (std_ss++holBACore_ss) [bir_bool_expTheory.bir_val_TF_bool2b_DEF] >>
+    PAT_X_ASSUM ``v1 <=+ A`` (MP_TAC) >>
+    REPEAT (POP_ASSUM (K ALL_TAC)) >>
+
+(*
+    now we are only left with the word relation
+*)
+
+    HolSmtLib.Z3_ORACLE_TAC
+*)
+  )
+QED
+(* ........................... *)
+
+
+
+
 
 Theorem abstract_jgmt_rel_incr[local]:
- abstract_jgmt_rel (bir_ts bir_incr_prog) (BL_Address (Imm64 0w)) {BL_Address (Imm64 8w)}
-  (\st. bir_exec_to_labels_triple_precond st bir_incr_pre bir_incr_prog)
-  (\st st'. bir_exec_to_labels_triple_postcond st' (\l. if l = BL_Address (Imm64 8w) then bir_incr_post else bir_exp_false) bir_incr_prog)
+ abstract_jgmt_rel (bir_ts bir_incr_prog) (BL_Address (Imm64 0w)) {BL_Address (Imm64 4w)}
+  (\st. bir_exec_to_labels_triple_precond st (bir_incr_pre pre_x10) bir_incr_prog)
+  (\st st'. bir_exec_to_labels_triple_postcond st' (\l. if l = BL_Address (Imm64 4w) then (bir_incr_post pre_x10) else bir_exp_false) bir_incr_prog)
 Proof
  (* reasoning via symb_prop_transfer_thm goes here *)
  cheat
@@ -177,15 +461,15 @@ QED
 
 Theorem bir_cont_incr[local]:
  bir_cont bir_incr_prog bir_exp_true (BL_Address (Imm64 0w))
-  {BL_Address (Imm64 8w)} {} bir_incr_pre
-  (\l. if l = BL_Address (Imm64 8w) then bir_incr_post else bir_exp_false)
+  {BL_Address (Imm64 4w)} {} (bir_incr_pre pre_x10)
+  (\l. if l = BL_Address (Imm64 4w) then (bir_incr_post pre_x10) else bir_exp_false)
 Proof
- `{BL_Address (Imm64 8w)} <> {}` by fs [] >>
+ `{BL_Address (Imm64 4w)} <> {}` by fs [] >>
  MP_TAC (Q.SPECL [`bir_incr_prog`,
   `BL_Address (Imm64 0w)`,
-  `{BL_Address (Imm64 8w)}`,
-  `bir_incr_pre`,
-  `\l. if l = BL_Address (Imm64 8w) then bir_incr_post else bir_exp_false`
+  `{BL_Address (Imm64 4w)}`,
+  `bir_incr_pre pre_x10`,
+  `\l. if l = BL_Address (Imm64 4w) then (bir_incr_post pre_x10) else bir_exp_false`
  ] abstract_jgmt_rel_bir_cont) >>
  rw [] >>
  METIS_TAC [abstract_jgmt_rel_incr]
